examples/Teleportation.v
@@ -1,57 +1,219 @@
 From Stdlib Require Import String.
-From Stdlib Require Lists.List.
-From Stdlib Require Import extraction.ExtrOcamlNativeString.
-Import List.ListNotations.
-
 From Qoreo Require Import Base Expr Choreography.
-From Qoreo Require Import Network NetQasm.
-From QoreoExamples Require Import Notation.
-Require Extraction.
-
-Import Choreography.
-Import ExampleNotation.
+From QoreoExamples Require Import HOASNotation.
 
 Open Scope string_scope.
+Open Scope example_scope.
 
-Module Teleportation.
-  Definition A : Actor.t := actor "alice"%string.
-  Definition B : Actor.t := actor "bob"%string.
 
-  Definition q : Var.t := var 0.
-  Definition a : Var.t := var 1.
-  Definition x : Var.t := var 2.
-  Definition z : Var.t := var 3.
-  Definition b : Var.t := var 4.
+Definition fresh_in_teleport q := q = 10.
 
-  Definition choreo : Choreography.t :=
-    [
-      (* Alice and Bob establish an entangled (EPR) pair. *)
-      epr{A, a; B, b};
+(* TODO: improve tactics for typechecking! *)
+Lemma WellTyped_teleport : forall Alice Bob q C,
+  Alice <> Bob ->
+  fresh_in_teleport q (* ensure q is fresh in teleport *) ->
+  WellTyped ChorEnv.empty (ChorEnv.add Bob q QUBIT ChorEnv.empty) ChorEnv.empty C ->
+  WellTyped ChorEnv.empty (ChorEnv.add Alice q QUBIT ChorEnv.empty) ChorEnv.empty
+    (mk (teleport Alice Bob q) ++ C)%list.
+Proof.
+  intros Alice Bob q C Hneq Hfresh HWT.
+  remember (mk (teleport Alice Bob q)) as C0 eqn:HC0.
+  cbv in HC0. subst.
+  unfold fresh_in_teleport in Hfresh; subst.
 
-      (* Alice performs some local operations and obtains classical bits x and z. *)
-      let{A, q := New[false]};
-      let{A, q := H[q]};
-      letp{A, (q, a) := CNOT[q, a]};
-      let!{A, x := Measure[q]};
-      let!{A, z := Measure[a]};
+  unfold ChorEnv.empty in *.
+  solve_wt ; ChorEnv.simplify.
 
-      (* Alice sends x and z to Bob. *)
-      send{A, x -> B, x};
-      send{A, z -> B, z};
+  econstructor.
+  { repeat (solve_wt; ChorEnv.simplify). }
+  2:{
+    ChorEnv.simplify.
+    Var.Map.Tactics.reflect_partition.
+    { apply Var.Map.Proofs.disjoint_empty_2. }
+    { Var.solve. }
+  }
+  2:{
+    Var.Map.Tactics.reflect_partition.
+    apply Var.Map.Proofs.disjoint_empty_2.
+    Var.solve.
+  }
+  2:{ Var.simplify. }
+  2:{ Var.simplify. }
+  2:{ auto. }
 
-      (* Bob uses x and z to update his qubit. *)
-      let{B, b := if_ (ref z) (Z[b]) (ref b)};
-      let{B, b := if_ (ref x) (X[b]) (ref b)};
-      let{B, b := H[b]}
-    ].
 
-  Definition parties : list Actor.t :=
-    [A; B].
+  ChorEnv.simplify.
+  right_associate Alice. ChorEnv.simplify. 
+  econstructor.
+  { repeat (solve_wt; ChorEnv.simplify). }
+  2:{
+    ChorEnv.simplify.
+    instantiate (1 := (Var.Map.add 3 QUBIT (Var.Map.empty typ))).
+    repeat (solve_wt; ChorEnv.simplify).
+  }
+  2:{
+    ChorEnv.simplify.
+    auto with var_db.
+  }
+  2:{ Var.simplify. }
 
-  Definition apps : option (list AppFile.t) :=
+  right_associate Alice. ChorEnv.simplify.
+  econstructor.
+  { repeat (solve_wt; ChorEnv.simplify). }
+  2:{
+    ChorEnv.simplify.
+    instantiate (1 := (Var.Map.add 3 QUBIT (Var.Map.empty typ))).
+    repeat (solve_wt; ChorEnv.simplify).
+  }
+  2:{ ChorEnv.simplify. auto with var_db. }
+  2:{ Var.simplify. }
+
+  right_associate Alice. ChorEnv.simplify.  
+
+  econstructor.
+  { repeat (solve_wt; ChorEnv.simplify). }
+  2:{
+    ChorEnv.simplify.
+    instantiate (1 := (Var.Map.add 5 (BANG BIT) (Var.Map.empty typ))).
+    repeat (solve_wt; ChorEnv.simplify).
+    rewrite Var.Map.Proofs.add_neq_sym; auto.
+    reflexivity.
+  }
+  2:{ ChorEnv.simplify. auto with var_db. }
+  2:{ Var.simplify. }
+
+  right_associate Alice. ChorEnv.simplify.
+
+  econstructor; auto.
+  { ChorEnv.simplify. repeat (solve_wt; ChorEnv.simplify). }
+  2:{
+    ChorEnv.simplify.
+    instantiate (1 := (Var.Map.add 6 (BANG BIT) (Var.Map.empty typ))).
+    repeat (solve_wt; ChorEnv.simplify).
+    Var.solve.
+  }
+  2:{ ChorEnv.simplify. auto with var_db. }
+
+  right_associate Alice. ChorEnv.simplify.
+  econstructor; auto.
+  { ChorEnv.simplify.
+    solve_wt.
+  }
+  2:{
+    ChorEnv.simplify.
+    instantiate (1 := (Var.Map.empty typ)).
+    repeat (solve_wt; ChorEnv.simplify).
+  }
+  2:{ ChorEnv.simplify. auto with var_db. }
+
+
+  right_associate Alice. ChorEnv.simplify.
+Require Import Lia.
+  econstructor; auto.
+  {
+    ChorEnv.simplify.
+    solve_wt.
+    { apply Expr.WTCVar; Var.simplify; eauto with var_db. }
+    { apply Expr.weakening. solve_wt. solve_wt; eauto with var_db.
+      Var.simplify. repeat solve_wt; auto with var_db. lia. lia.
+    } 
+    { apply Expr.weakening. solve_wt.
+      Var.simplify. repeat solve_wt; auto with var_db. lia. lia.
+    }
+    { auto with var_db. }
+    { auto with var_db. }
+  }
+  2:{
+    ChorEnv.simplify.
+    auto with var_db.
+  }
+  2:{ ChorEnv.simplify. auto with var_db. }
+  2:{ Var.simplify. }
+
+  ChorEnv.simplify. simpl.
+  econstructor; auto.
+  {
+    ChorEnv.simplify.
+    solve_wt.
+    { apply Expr.WTCVar; Var.simplify; eauto with var_db. }
+    { apply Expr.weakening. solve_wt. simpl. solve_wt; eauto with var_db.
+      Var.simplify. repeat solve_wt; auto with var_db. lia.
+    } 
+    { apply Expr.weakening. solve_wt.
+      Var.simplify. repeat solve_wt; auto with var_db. lia.
+    }
+    { auto with var_db. }
+    { auto with var_db. }
+  }
+  2:{
+    ChorEnv.simplify.
+    auto with var_db.
+  }
+  2:{ ChorEnv.simplify. auto with var_db. }
+  2:{ Var.simplify. }
+
+  unfold ChorEnv.remove. ChorEnv.simplify.
+
+  eapply Choreography.weakening_gen with (G := Actor.Map.empty (Var.Map.t typ)) (G0 := ChorEnv.add Bob 8 BIT (ChorEnv.add Bob 7 BIT (Actor.Map.empty _))).
+  2:{
+    intros B. split. ChorEnv.simplify; auto with var_db.
+    ChorEnv.simplify. repeat solve_wt; auto with var_db; lia.
+  }
+
+  ChorEnv.simplify.
+  assert (Heq' :ChorEnv.Equal (Actor.Map.remove Alice (Actor.Map.empty (Var.Map.t typ)))
+                (Actor.Map.empty (Var.Map.t typ))).
+  { ChorEnv.solve. }
+  rewrite Heq'; clear Heq'.
+
+  auto.
+Qed.
+
+Definition choreo : Choreography.t :=
+  mk (
+    do q ← "alice" [- Unitary H (New (Bit false))-] ;;
+    teleport "alice" "bob" q
+  ).
+
+Eval compute in choreo.
+
+Eval compute in (Network.epp "alice" choreo).
+(*
+  do q ← Unitary H (New (Bit false)) ;;
+  do a ← establish_entanglement Bob ;;
+  do (q,a) ← Unitary CNOT (q,a) ;;
+  do q ← unitary H q ;;
+  do x ← Meas q ;;
+  do z ← Meas a ;;
+  do _ ← Send Bob x ;;
+  Send Bob z
+*)
+
+
+Eval compute in (Network.epp "bob" choreo).
+(*
+  do b ← establish_entanglement Alice ;;
+  do x ← Receive Alice ;;
+  do z ← Receive Alice ;;
+  do b ← If z (Unitary Z b) b ;;
+  If x (Unitary X b) b
+*)
+
+
+Eval compute in (Network.epp "bob" choreo).
+
+
+Definition parties : list Actor.t :=
+  ["alice"; "bob"].
+
+
+Import ExampleExtraction.
+From Stdlib Require Import extraction.ExtrOcamlNativeString.
+From Qoreo Require Import NetQasm.
+
+Definition apps : option (list AppFile.t) :=
     ExampleExtraction.render_parties choreo parties.
-End Teleportation.
 
 Extraction Language OCaml.
 Set Extraction Output Directory "extracted".
-Extraction "teleportation_netqasm.ml" Teleportation.apps.
+Extraction "teleportation_netqasm.ml" apps.
