examples/OldNotation.v/Notation.v
@@ -1,0 +1,80 @@
+From Stdlib Require Import String.
+From Stdlib Require Lists.List.
+Import List.ListNotations.
+
+From Qoreo Require Import Base Expr Choreography Network NetQasm.
+
+Open Scope string_scope.
+
+Module ExampleNotation.
+  Import Choreography.
+
+  Definition actor (name : string) : Actor.t := name.
+  Definition var (n : nat) : Var.t := n.
+
+  Definition ref (x : Var.t) : Expr.t := Expr.Var x.
+
+  Definition measure (x : Var.t) : Expr.t :=
+    Expr.Meas (ref x).
+
+  Definition new (b : bool) : Expr.t :=
+    Expr.New (Expr.Bit b).
+
+  Definition apply1 (u : unitary) (x : Var.t) : Expr.t :=
+    Expr.Unitary u (ref x).
+
+  Definition apply2 (u : unitary) (x y : Var.t) : Expr.t :=
+    Expr.Unitary u (Expr.Pair (ref x) (ref y)).
+
+  Definition if_ (cond_ then_ else_ : Expr.t) : Expr.t :=
+    Expr.If cond_ then_ else_.
+
+  Notation "'epr{' A ',' x ';' B ',' y '}'" := (Choreography.Insn.EPR A x B y)
+    (at level 0, x at next level, y at next level).
+
+  Notation "'send{' A ',' x '->' B ',' y '}'" := (Choreography.Insn.Send A (ref x) B y)
+    (at level 0, x at next level, y at next level).
+
+  Notation "'let{' A ',' x ':=' e '}'" := (Choreography.Insn.Let A x e)
+    (at level 0, x at next level, e at next level).
+
+  Notation "'let!{' A ',' x ':=' e '}'" := (Choreography.Insn.LetBang A x e)
+    (at level 0, x at next level, e at next level).
+
+  Notation "'letp{' A ',' '(' x ',' y ')' ':=' e '}'" := (Choreography.Insn.LetPair A x y e)
+    (at level 0, x at next level, y at next level, e at next level).
+
+  Notation "'H[' x ']'" := (apply1 H x)
+    (at level 0, x at next level).
+  Notation "'X[' x ']'" := (apply1 X x)
+    (at level 0, x at next level).
+  Notation "'Z[' x ']'" := (apply1 Z x)
+    (at level 0, x at next level).
+  Notation "'CNOT[' x ',' y ']'" := (apply2 CNOT x y)
+    (at level 0, x at next level, y at next level).
+  Notation "'Measure[' x ']'" := (measure x)
+    (at level 0, x at next level).
+  Notation "'New[' b ']'" := (new b)
+    (at level 0, b at next level).
+End ExampleNotation.
+
+Module ExampleExtraction.
+  Definition render_party (choreo : Choreography.t) (p : Actor.t)
+    : option AppFile.t :=
+    match Network.epp p choreo with
+    | Some proc =>
+        Some {| AppFile.party := p; AppFile.source := render_app p proc |}
+    | None => None
+    end.
+
+  Fixpoint render_parties (choreo : Choreography.t) (ps : list Actor.t)
+    : option (list AppFile.t) :=
+    match ps with
+    | [] => Some []
+    | p :: ps' =>
+        match render_party choreo p, render_parties choreo ps' with
+        | Some app, Some apps => Some (app :: apps)
+        | _, _ => None
+        end
+    end.
+End ExampleExtraction.
