src/Expr.v
@@ -1,3 +1,24 @@
+(**
+  Definition of the local quantum expression language
+
+  Data structures:
+
+  - `Expr.t` - Qoreo AST
+  - `Expr.step` - small-step operational semantics
+  - `Expr.typ` - Qoreo types
+  - `Expr.WellTyped` - typing relation
+
+  Theorems:
+
+  - `wt_subst`, `wt_subst_bang`: substitution lemmas for linear and non-linear variables respectively
+  - `WellTyped_preservation`: preservation of the typing relation with respect to the step relation
+  - `WellScoped_preservation`: preservation of the configuration well-scopedness relation with respect to the step relation
+  - `preservation`: conjunction of the previous two lemmas
+  - 'progress': well-typed terms are either values or can take a step
+  - `safety`: top-level type safety theorem
+
+  *)
+
 From Stdlib Require Import FSets.FMapList FSets.FSetList FSets.FMapFacts OrderedType OrderedTypeEx.
 From QuantumLib Require Import Matrix Pad Quantum.
 From Qoreo Require Import Base.
