README.md
@@ -12,20 +12,81 @@ Qoreo uses the QuantumLib library for formalizing quantum computing (https://git
 opam pin coq-quantumlib https://github.com/jpaykin/QuantumLib.git#jpaykin/v9.1
 ```
 
-Once dependencies have been installed, build the Qoreo repository using `make`. The workflow uses CoqMakefile.
+Once dependencies have been installed, you can build the Rocq proofs using `make proofs`. The workflow uses CoqMakefile.
+
 
 # Structure
+
+The repository is organized in 4 main directories.
+
+* `src` - Rocq implementation of Qoreo
+    - `src/Base.v` - Definition of common structures used in the formaliztion
+        - `FMap` - finite maps
+        - `Var` - variables represented as natural numbers
+        - `unitary` - data structure of unitary gates
+        - `Config` - quantum states represented as QuantumLib density matrices
+        - `Actor` - actors in a network, represented as strings
+        - `ChorEnv` - specialized finite maps from pairs of actors and variable names.
+
+    - `src/Expr.v` - Definition of the local quantum expression language
+        - `Expr.t` - Qoreo AST
+        - `Expr.step` - small-step operational semantics
+        - `Expr.typ` - Qoreo types
+        - `Expr.WellTyped` - typing relation
+        - `wt_subst`, `wt_subst_bang` - substitution lemmas for linear and non-linear variables respectively
+        - `WellTyped_preservation` - preservation of the typing relation with respect to the step relation
+        - `WellScoped_preservation` - preservation of the configuration well-scopedness relation with respect to the step relation
+        - `preservation`- conjunction of the previous two lemmas
+        - 'progress' - well-typed terms are either values or can take a step
+        - `safety` - top-level type safety theorem
+
+    - `src/Choreography.v` - Definition of the choreographic language
+        - `Insn.t`, `Expr.t` - Choreographic instructions and choreographies, respectively
+        - `step` - small-step operational semantics
+        - `WellTyped` - typing relation
+        - `wt_subst_lin`, `wt_subst_bang`: substitution lemmas for linear and non-linear variables respectively
+        - `WellTyped_preservation`: preservation of the typing relation with respect to the step relation
+        - `WellScoped_preservation`: preservation of the configuration well-scopedness relation with respect to the step relation
+        - `preservation`: conjunction of the previous two lemmas
+        - 'progress': well-typed choreographies are either values or can take a step
+        - `safety`: top-level type safety theorem
+
+
+    - `src/Network.v`: Definition of process language and endpoint projection
+        - `Insn.t`, `Process.t`, `Network.t` - Definiton of choreographic instructions, processes, and networks respectively
+        - `Process.step`, `Network.step` - small-step operational semantics
+        - `epp` - Definition of endpoint projection as a function from choreographies and an actor name to a process.
+        - `EPP` - Relational definition of endpoint projection
+        - `EPP_N` - Relational definition of when a choreography is projected onto an entire network
+        - `soundness` - Soundness of EPP; if a choreography can take a step, then so can the projected choreography
+        - `completeness` - Completeness of EPP; if a projected choreography can take a step, then so can the unprojected choreography
+        - `safety` - Well-typed choreographies project to safe and deadlock-free networks
+
+    - `src/NetQasm.v` - Render Qoreo processes as NetQASM strings
+
+* `examples/`
+
+    - `examples/Notation.v` - Introduces a Qoreo construction DSL monad that uses higher-order abstract syntax (HOAS) to construct choreographies in a natural style
+
+    - `examples/MeasureSend.v` - trivial examples that measures a qubit and sends it on a channel
+    - `examples/Teleportation.v` - choreographic implementation of quantum teleportation
+    - `examples/Protocols.v` - a variety of protocols including distributed controlled-unitaries and a distributed VQA pass
+    - `examples/b92.v` - implementaiton of B92 quantum key distribution algorithm
+
+        * `test_examples/test_b92.py` - python instrumentation for B91
+
+* `ocaml/` - A directory that instrments the extracted ocaml code for each examples
+
+* `python/ocaml_netqasm_runtime.py` - Implementation of a simple python runtime library using netqasm.
+
+
+# Contributing to the repository
 
 To add a new Rocq `.v` file, add it to the `src/` subdirectory and add it to the list of filenames in the `_CoqProject` file.
 
 Qoreo uses the OCaml/Rocq concept of modules to define data structures. The variables in `src/Base.v` are a good example: they are defined in a module `Var`, and the type of such variables is `Var.t`. Other helper functions such as decidable equality of variables are also defined in this module (`Var.eq_dec`). Modules can be nested, e.g. `Var.FSet.t` is the type of finite sets of variables.
 
-* `src/Base.v` - Variables `Var.t`; quantum references `qref` and unitaries; quantum states `Config.t`; and actors `Actor.t`.
-* `src/Expr.v` - The definition of the local quantum language language.
-* `src/Choreography.v` - The definition of the choreographic language.
-* `src/Network.v` - The definition of the network language.
-
-# Compiling to NetQASM
+# Extracting to NetQASM
 
 The `examples` directory includes:
 
